LearnLean/FunctionalProgramming/3_FastIntro/5_proofs.lean
@@ -1,0 +1,37 @@
+set_option autoImplicit true
+#check rfl
+
+def x : 1=1 := rfl
+
+def OnePlusOneIsTwo : Prop := 1 + 1 = 2
+
+#check OnePlusOneIsTwo
+
+theorem onePlusOneIsTwo : OnePlusOneIsTwo := rfl
+
+#check onePlusOneIsTwo
+
+theorem _onePlusOneIsTwo : 1 + 1 = 2 := by
+  simp
+
+#check _onePlusOneIsTwo
+
+def third (xs : List α) (ok : xs.length > 2) : α := xs[2]
+
+def woodlandCritters : List String :=
+  ["hedgehog", "deer", "snail"]
+
+#eval third woodlandCritters (by decide)
+
+def l : List Nat := [1,2,3]
+
+theorem ok: l.length > 2 := by decide
+
+#eval third l (by decide)
+
+
+-- #eval l[2]
+
+def thirdOption (xs : List α) : Option α := xs[2]?
+
+#eval thirdOption woodlandCritters
