LearnLean/FunctionalProgramming/3_FastIntro/6_typeclass.lean
@@ -1,0 +1,76 @@
+class Plus (α : Type) where
+  plus : α → α → α
+
+instance : Plus Nat where
+  plus := Nat.add
+
+instance : Plus String where
+  plus := String.append
+
+instance {α : Type} : Plus (List α) where
+  plus := List.append
+
+open Plus (plus)
+
+#eval plus 5 3
+#eval plus "Ok" "my"
+#eval plus [1,2] [3,4]
+
+
+inductive Pos : Type where
+  | one : Pos
+  | succ (p : Pos)
+
+-- def toNat (p : Pos) : Nat :=
+--   match p with
+--   | Pos.one => 0
+--   | Pos.succ p => Nat.succ (toNat p)
+
+def toNat : Pos → Nat
+  | Pos.one => 1
+  | Pos.succ p => Nat.succ (toNat p)
+
+def p := Pos.succ (Pos.succ Pos.one)
+def q := Pos.succ (Pos.succ (Pos.succ Pos.one))
+
+def Pos.plus : Pos → Pos → Pos
+  | Pos.one, q => Pos.succ q
+  | Pos.succ p, q =>  Pos.succ (Pos.plus p q)
+
+instance : Plus Pos where
+  plus := Pos.plus
+#eval p
+#eval toNat p
+#eval toNat (plus p p)
+#eval toNat (plus p q)
+
+instance : Add Pos where
+  add := Pos.plus
+
+#eval p + q
+
+def posToString : Pos → String
+  | p => toString (toNat p)
+
+instance : ToString Pos where
+  toString := posToString
+
+#eval p + q
+
+-- class OfNat (α : Type) (_ : Nat) where
+--   ofNat : α
+
+-- instance : OfNat Pos 1 where
+--   ofNat := Pos.one
+-- instance : OfNat Pos 2 where
+--   ofNat := Pos.succ Pos.one
+
+instance {n : Nat} : OfNat Pos (n + 1) where
+  ofNat :=
+    let rec natPlusOne : Nat → Pos
+      | 0 => Pos.one
+      | k + 1 => Pos.succ (natPlusOne k)
+    natPlusOne n
+
+
+def x : Pos := 2
