LearnLean/FunctionalProgramming/3_FastIntro/7_typeclasspolymorphism.lean
@@ -1,0 +1,104 @@
+-- set_option autoImplicit true
+
+structure Point (α : Type) where
+  x : α
+  y : α
+deriving Repr
+
+def Point.P (u:Unit) : Point Float := {x:=0.0, y:=0.0}
+
+instance {α : Type} [Add α] : Add (Point α) where
+  add p1 p2 := { x:= p1.x + p2.x, y:= p1.y + p2.y }
+
+
+def p1 : Point Float := ⟨1,2⟩
+def p2 : Point Float := ⟨1,0⟩
+#eval p1
+#eval p1 + p2
+
+#check ()
+#eval {x := 2, y:=2 : Point Float}
+
+-- close the open
+namespace Point
+#eval P ()
+end Point
+
+#check Point
+
+#check @OfNat.ofNat
+
+
+inductive Even where
+  | zero : Even
+  | succ : Even → Even
+
+-- instance {n : Nat} : OfNat Even n where
+--   ofNat :=
+--     let rec natPlusOne : Nat → Even
+--       | 0 => Even.zero
+--       | k => Even.succ (natPlusOne k) + 2
+--     natPlusOne n
+
+
+instance : OfNat Even 0 where
+  ofNat := Even.zero
+
+instance {n : Nat} [OfNat Even n] : OfNat Even (n+2) where
+  ofNat := Even.succ (OfNat.ofNat n)
+
+def exampleEven : Even := OfNat.ofNat 4
+#eval exampleEven
+
+def z : Even := 0
+#eval z
+
+-- def three : Even := 3
+-- #eval three
+
+def two : Even := 2
+#eval two
+def four : Even := 4
+#eval four
+
+def many : Even := 254
+#eval 254/2
+
+def Even.toNat : Even → Nat
+  | Even.zero => 0
+  | Even.succ s => 2 + Even.toNat s
+
+def isEven : Nat → Bool
+  | 0 => true
+  | 1 => false
+  | n + 2 => isEven n
+
+#eval Even.toNat two
+#eval Even.toNat four
+
+
+def Even.plus : Even → Even → Even
+  | Even.zero, e => e
+  | Even.succ s, e => Even.plus s (Even.succ e)
+
+#eval Even.plus two two
+#eval Even.toNat (Even.plus two two)
+#eval Even.toNat (Even.plus two four)
+
+instance : Add Even where
+  add := Even.plus
+
+def Even.mul : Even → Even → Even
+  | Even.zero, _ => Even.zero
+  | Even.succ s, e => (Even.plus e (Even.mul s e)) + e
+
+
+#eval Even.toNat (four + two + two)
+#eval Even.toNat (four + four)
+#eval Even.toNat (Even.mul two four)
+#eval Even.toNat (Even.mul four four)
+#eval Even.toNat (Even.mul four two)
+#eval Even.toNat (Even.mul two (Even.mul four four))
+#eval Even.toNat (Even.mul four (Even.mul four four))
+#eval Even.toNat (Even.mul Even.zero (Even.mul four four))
+#eval Even.toNat (Even.mul four Even.zero)
