LearnLean/FunctionalProgramming/3_FastIntro/8_control.lean
@@ -1,0 +1,109 @@
+inductive Pos : Type where
+  | one : Pos
+  | succ (p : Pos)
+
+def addNatPos : Nat → Pos → Pos
+  | 0, p => p
+  | n + 1, p => Pos.succ (addNatPos n p)
+
+def addPosNat : Pos → Nat → Pos
+  | p, 0 => p
+  | p, n + 1 => Pos.succ (addPosNat p n)
+
+instance {n : Nat} : OfNat Pos (n + 1) where
+  ofNat :=
+    let rec natPlusOne : Nat → Pos
+      | 0 => Pos.one
+      | k + 1 => Pos.succ (natPlusOne k)
+    natPlusOne n
+
+
+class HPlus (α : Type) (β : Type) (γ : Type) where
+  hPlus : α → β → γ
+
+instance : HPlus Nat Pos Pos where
+  hPlus := addNatPos
+
+instance : HPlus Pos Nat Pos where
+  hPlus := addPosNat
+
+#eval (HPlus.hPlus (3 : Pos) (5 : Nat) : Pos)
+
+-- #eval HPlus.hPlus (3 : Pos) (5 : Nat)
+-- The commented code above does not work. Why?
+-- Because HPlus signature has two input types and an output type
+-- Thus, we can declare another behavior where the output is something different
+
+instance : HPlus Pos Nat String where
+  hPlus := fun x y => "eyo"
+
+#eval (HPlus.hPlus (3 : Pos) (5 : Nat) : String)
+
+
+namespace HPlus2
+-- We can avoid having to pass the output type using outParam
+-- outParam is a special annotation that indicates
+-- that a type is an output parameter of a function.
+-- Hence, this gives more context for Lean to
+-- infer which type this should be.
+-- Note that this allows us to write our function
+-- without writing the specific type, even when we have
+-- ambiguity. Check the example below:
+class HPlus (α : Type) (β : Type) (γ : outParam Type) where
+  hPlus : α → β → γ
+
+instance : HPlus Pos Nat String where
+  hPlus := fun x y => "ok"
+
+instance : HPlus Nat Pos Pos where
+  hPlus := addNatPos
+
+instance : HPlus Pos Nat Pos where
+  hPlus := addPosNat
+
+#eval HPlus.hPlus (3 : Pos) (5 : Nat)
+
+-- The output above uses the Pos → Nat → Pos, instead of the Pos → Nat → String
+-- Why? Because Lean tries to infer what makes more "sense" in the context.
+-- Since Pos is already in the input type, then the probable "default"
+-- output type is the Pos, instead of String.
+
+instance : HPlus Pos Nat Nat where
+  hPlus := fun x y => 0
+
+#eval HPlus.hPlus (3 : Pos) (5 : Nat)
+-- If we also declare a Pos → Nat → Nat, the new default becomes the output Nat.
+end HPlus2
+
+-- At last, we can control this default type.
+-- But one must be careful! As this might lead to confusing type inference.
+namespace HPlus3
+
+@[default_instance]
+instance {α : Type} [Add α] : HPlus α α α where
+  hPlus := Add.add
+
+#check HPlus.hPlus 2
+-- It returns a type Nat → Nat, because it assumes that the
+-- default output type will be the same as the input.
+
+end HPlus3
+
+namespace HPlus4
+
+class HPlus (α : Type) (β : Type) (γ : outParam Type) where
+  hPlus : α → β → γ
+
+@[default_instance]
+instance : HPlus Pos Nat String where
+  hPlus := fun x y => "ok"
+
+instance : HPlus Pos Nat Pos where
+  hPlus := addPosNat
+
+#check HPlus.hPlus (2 : Pos)
+
+#eval HPlus.hPlus (2 : Pos) 2
+#eval HPlus.hPlus (2 : Pos) (2 :Nat)
+
+end HPlus4
